prove time bounds on ipow
this gigantic monolithic commit (oops) also includes:

 * adaptation of straightline for metric-aware proofs
 * adaptation of some tail recursion proofs; many are commented out
 * various utilities for arithmetic on MetricLogs

bedrock2/src/bedrock2Examples/ipow.v
@@ -1,5 +1,6 @@
 Require Import Coq.ZArith.ZArith coqutil.Z.div_mod_to_equations.
 Require Import bedrock2.NotationsCustomEntry.
+Require Import bedrock2.MetricLogging.
 Import Syntax BinInt String List.ListNotations ZArith.
 Require Import coqutil.Z.Lia.
 Local Open Scope string_scope. Local Open Scope Z_scope. Local Open Scope list_scope.
@@ -20,13 +21,22 @@ Definition ipow :=
 From bedrock2 Require Import Semantics BasicC64Semantics WeakestPrecondition ProgramLogic.
 From coqutil Require Import Word.Properties Word.Interface Tactics.letexists.
 
-Instance spec_of_ipow : spec_of "ipow" := fun functions =>
-  forall x e t m,
-    WeakestPrecondition.call functions
-      "ipow" t m [x; e]
-      (fun t' m' rets => t=t'/\ m=m' /\ exists v, rets = [v] /\ (
-        word.unsigned v = word.unsigned x ^ word.unsigned e mod 2^width)).
+Definition initCost := {| instructions := 9; stores := 0; loads := 9; jumps := 0 |}.
+Definition iterCost := {| instructions := 38; stores := 0; loads := 45; jumps := 2 |}.
+Definition endCost :=  {| instructions := 2; stores := 0; loads := 3; jumps := 1 |}.
 
+Definition msb z := match z with
+                    | Zpos _ => Z.log2 z + 1
+                    | _ => 0
+                    end.
+
+Instance spec_of_ipow : spec_of "ipow" := fun functions =>
+  forall x e t m mc,
+    WeakestPrecondition.call functions
+      "ipow" t m [x; e] mc
+      (fun t' m' rets mc' => t=t'/\ m=m' /\ exists v, rets = [v] /\ (
+        word.unsigned v = word.unsigned x ^ word.unsigned e mod 2^width) /\
+        (mc' - mc <= initCost + (msb (word.unsigned e)) * iterCost + endCost)%metricsH).
 
 Module Z.
   Lemma pow_mod x n m (Hnz: m <> 0) : (x mod m)^n mod m = x^n mod m.
@@ -64,6 +74,34 @@ Ltac t :=
   repeat match goal with H: absint_eq ?x ?x |- _ => clear H end;
   cbv [absint_eq] in *.
 
+Lemma msb_shift z : 0 < z -> msb (z / 2) = msb z - 1.
+Proof.
+  intro.
+  case (z / 2) eqn:Hdiv.
+  - enough (H1 : z = 1) by (rewrite H1; easy).
+    enough (z = z mod 2) by (Z.div_mod_to_equations; blia).
+    rewrite (Z.div_mod z 2) by blia.
+    rewrite Hdiv.
+    cbn.
+    rewrite Zmod_mod.
+    reflexivity.
+  - rewrite <- Z.div2_div in Hdiv.
+    rewrite (Zdiv2_odd_eqn z).
+    rewrite Hdiv.
+    rewrite <- Pos2Z.inj_mul.
+    case (Z.odd z);
+    [rewrite <- Pos2Z.inj_add | rewrite Z.add_0_r];
+    unfold msb;
+    rewrite Z.add_simpl_r;
+    [rewrite Pos2Z.inj_add |]; rewrite Pos2Z.inj_mul;
+    [rewrite Z.log2_succ_double | rewrite Z.log2_double];
+    blia.
+  - pose proof (Zlt_neg_0 p) as Hneg.
+    rewrite <- Hdiv in Hneg.
+    Z.div_mod_to_equations.
+    blia.
+Qed.
+
 Lemma ipow_ok : program_logic_goal_for_function! ipow.
 Proof.
   repeat straightline.
@@ -71,9 +109,10 @@ Proof.
   refine ((TailRecursion.tailrec
     (* types of ghost variables*) HList.polymorphic_list.nil
     (* program variables *) (["e";"ret";"x"] : list String.string))
-    (fun v t m e ret x => PrimitivePair.pair.mk (v = word.unsigned e) (* precondition *)
-    (fun   T M E RET X => T = t /\ M = m /\ (* postcondition *)
-        word.unsigned RET = word.unsigned ret * word.unsigned x ^ word.unsigned e mod 2^width))
+    (fun v t m e ret x mc => PrimitivePair.pair.mk (v = word.unsigned e) (* precondition *)
+    (fun   T M E RET X MC => T = t /\ M = m /\ (* postcondition *)
+        word.unsigned RET = word.unsigned ret * word.unsigned x ^ word.unsigned e mod 2^width /\
+        (MC - mc <= msb (word.unsigned e) * iterCost + endCost)%metricsH))
     (fun n m => 0 <= n < m) (* well_founded relation *)
     _ _ _ _ _);
     (* TODO wrap this into a tactic with the previous refine *)
@@ -91,13 +130,13 @@ Proof.
   { (* loop test *)
     repeat straightline; try show_program.
     { (* loop body *)
-      letexists; split; [repeat straightline|]. (* if condition evaluation *)
+      eexists; eexists; split; [repeat straightline|]. (* if condition evaluation *)
       split. (* if cases, path-blasting *)
       {
-        repeat (straightline || (split; trivial; [])). all:t.
+        repeat (straightline || (split; trivial; [])). 2: split. all:t.
         { (* measure decreases *)
           set (word.unsigned x0) in *. (* WHY does blia need this? *)
-          Z.div_mod_to_equations; blia. }
+          Z.div_mod_to_equations. blia. }
         { (* invariant preserved *)
           rewrite H3; clear H3. rename H0 into Hbit.
           change (1+1) with 2 in *.
@@ -112,10 +151,22 @@ Proof.
           rewrite ?Z.pow_add_r by (pose proof word.unsigned_range x0; Z.div_mod_to_equations; blia).
           rewrite ?Z.pow_twice_r, ?Z.pow_1_r, ?Z.pow_mul_l.
           rewrite Z.mul_mod_idemp_r by discriminate.
-          f_equal; ring. } }
+          f_equal; ring. }
+        { (* metrics correct *)
+          cbn [addMetricLoads withLoads instructions stores loads jumps] in H4.
+          applyAddMetrics H4.
+          rewrite msb_shift in H4 by blia.
+          rewrite MetricArith.mul_sub_distr_r in H4.
+          rewrite <- MetricArith.add_sub_swap in H4.
+          rewrite <- MetricArith.le_add_le_sub_r in H4.
+          eapply MetricArith.le_trans.
+          2: exact H4.
+          unfold iterCost.
+          solve_MetricLog.
+        }
+      }
       {
-        repeat (straightline || (split; trivial; [])).
-        all: t.
+        repeat (straightline || (split; trivial; [])). 2: split. all: t.
         { (* measure decreases *)
           set (word.unsigned x0) in *. (* WHY does blia need this? *)
           Z.div_mod_to_equations; blia. }
@@ -130,11 +181,42 @@ Proof.
           rewrite <-(Z.mul_mod_idemp_r _ (_^_)), Z.pow_mod by discriminate.
           rewrite ?Z.add_0_r, Z.pow_twice_r, ?Z.pow_1_r, ?Z.pow_mul_l.
           rewrite Z.mul_mod_idemp_r by discriminate.
-          f_equal; ring. } } }
-    { (* postcondition *) rewrite H, Z.pow_0_r, Z.mul_1_r, word.wrap_unsigned; auto. } }
+          f_equal; ring. }
+        { (* metrics correct *)
+          cbn [addMetricLoads withLoads instructions stores loads jumps] in H4.
+          applyAddMetrics H4.
+          rewrite msb_shift in H4 by blia.
+          rewrite MetricArith.mul_sub_distr_r in H4.
+          rewrite <- MetricArith.add_sub_swap in H4.
+          rewrite <- MetricArith.le_add_le_sub_r in H4.
+          eapply MetricArith.le_trans.
+          2: exact H4.
+          unfold iterCost.
+          solve_MetricLog.
+        }
+      }
+    }
+    { (* postcondition *)
+      rewrite H, Z.pow_0_r, Z.mul_1_r, word.wrap_unsigned.
+      repeat match goal with
+             | |- _ /\ _ => split
+             | |- _ = _ => reflexivity
+             end.
+      unfold msb, iterCost, endCost.
+      subst mc'.
+      solve_MetricLog.
+    }
+  }
 
   repeat straightline.
+  repeat match goal with
+         | |- _ /\ _ => split
+         | |- _ = _ => reflexivity
+         | |- exists _, _ => letexists
+         | _ => t
+         end.
+  1: setoid_rewrite H1; setoid_rewrite Z.mul_1_l; trivial.
 
-  repeat (split || letexists || t || trivial).
-  setoid_rewrite H1; setoid_rewrite Z.mul_1_l; trivial.
-Defined.
+  unfold initCost, iterCost, endCost in *.
+  solve_MetricLog.
+Qed.
